SStructTT/SStruct/Static/Typed.lean
@@ -1,16 +1,16 @@
-import SStructTT.Defs.SStruct
-import SStructTT.Defs.Syntax
-import SStructTT.Static.Confluence
-import SStructTT.Static.Context
+import SStructTT.SStruct.Syntax
+import SStructTT.SStruct.SrtOrder
+import SStructTT.SStruct.Static.Confluence
+import SStructTT.SStruct.Static.Context
 
 namespace Static
-variable {Srt : Type} [SStruct Srt]
+variable {Srt : Type} [ord : SrtOrder Srt]
 
 mutual
 inductive Typed : Ctx Srt -> Tm Srt -> Tm Srt -> Prop where
   | srt {Γ} s i :
     Wf Γ ->
-    Typed Γ (.srt s i) (.srt s0 (i + 1))
+    Typed Γ (.srt s i) (.srt ord.s0 (i + 1))
 
   | var {Γ x A} :
     Wf Γ ->
@@ -53,7 +53,7 @@ inductive Typed : Ctx Srt -> Tm Srt -> Tm Srt -> Prop where
 
   | bool {Γ} :
     Wf Γ ->
-    Typed Γ .bool (.srt s0 0)
+    Typed Γ .bool (.srt ord.s0 0)
 
   | tt {Γ} :
     Wf Γ ->
@@ -74,7 +74,7 @@ inductive Typed : Ctx Srt -> Tm Srt -> Tm Srt -> Prop where
     Typed Γ A (.srt s i) ->
     Typed Γ m A ->
     Typed Γ n A ->
-    Typed Γ (.idn A m n) (.srt s0 i)
+    Typed Γ (.idn A m n) (.srt ord.s0 i)
 
   | rfl {Γ A m} :
     Typed Γ m A ->
